Some examples

Flow.v
@@ -4,10 +4,11 @@ From Coq Require Import FunctionalExtensionality PropExtensionality.
 From CDF Require Import Sequences Separation Seplog.
 
 Local Open Scope string_scope.
-Local Open Scope nat_scope.
+(* Local Open Scope nat_scope. *)
+Local Open Scope Z_scope.
 Local Open Scope list_scope.
 
-Section Flow.
+Module Flow.
 
 Definition flow : Type := heap -> heap -> Prop.
 
@@ -61,13 +62,13 @@ Inductive forward : com -> flow -> Prop :=
 
   .
 
-Inductive satisfies : heap -> flow -> heap -> Prop :=
+(* this axiomatization of the models relation is not needed because of the semantic definitions above *)
+(* Inductive satisfies : heap -> flow -> heap -> Prop :=
   | m_req: forall h1 h2 p k,
     satisfies h1 (freq p k) h2
   | m_ens: forall h1 h2 q,
     satisfies h1 (fens q) h2
-
-.
+. *)
 
 (* Example e1 : forall h1 h2, red (PURE 0, h1) (PURE 0, h2).
 intros.
@@ -101,7 +102,7 @@ Definition terminates (c1: com) (h1 h2: heap) : Prop :=
 Theorem soundness : forall f c1 h1 h2 h3,
   forward c1 f ->
   terminates c1 h1 h2 ->
-  satisfies h1 f h3 ->
+  f h1 h3 ->
   h2 = h3.
 Proof.
 admit.
@@ -151,3 +152,272 @@ Qed.
 (* Admitted. *)
 
 End Flow.
+
+Module Flow2.
+
+  Definition flow : Type := heap -> heap -> bool -> Z -> Prop.
+
+  Definition fexists {A: Type} (P: A -> flow) : flow :=
+    fun h1 h2 p r =>
+      exists a: A, P a h1 h2 p r.
+    
+  (* h3 is the part of the heap that is taken away by req,
+    h4 is what is left *)
+  Definition freq (P: precond) : flow :=
+    fun h1 h2 p r =>
+        (exists h3 h4, h1 = hunion h3 h4
+          /\ hdisjoint h3 h4
+          /\ P h3 /\ h2 = h4 /\ p = true)
+        \/
+        (forall h3 h4, h1 = hunion h3 h4
+          /\ hdisjoint h3 h4
+          /\ not (P h3) -> p = false).
+
+  Definition fens (P: postcond) : flow :=
+    fun h1 h2 p r =>
+      exists h3,
+        P r h3
+        /\ h2 = hunion h1 h3
+        /\ hdisjoint h1 h3.
+
+  Definition fempty : flow := fens (fun r h => h = hempty).
+
+  Definition fseq (f1 f2 : flow) : flow :=
+    fun h1 h2 p r =>
+        (exists h3 r1,
+          f1 h1 h3 true r1 /\ f2 h3 h2 p r)
+        \/ f1 h1 h2 false r.
+
+  Infix ";;" := fseq (at level 80, right associativity).
+
+  Example ex_take_put_back : forall x v r, (freq (contains x v) ;; fens (fun r => contains x v)) (hupdate x v hempty) (hupdate x v hempty) true r.
+  Proof.
+    intros.
+    unfold fseq.
+    left.
+    exists hempty. exists 1.
+    split.
+    - unfold freq.
+    left.
+    exists (hupdate x v hempty).
+    exists hempty.
+    split.
+    rewrite <- hunion_comm.
+    rewrite hunion_empty.
+    reflexivity.
+    rewrite hdisjoint_sym.
+    apply hdisjoint_empty.
+    split.
+    HDISJ.
+    split.
+    unfold contains.
+    reflexivity.
+    split; auto.
+    - unfold fens.
+    exists (hupdate x v hempty).
+    repeat split.
+    rewrite hunion_empty.
+    reflexivity.
+    apply hdisjoint_empty.
+  Qed.
+
+  Example ex_vacuous_req : forall x v r, (freq (contains x v)) (hempty) (hupdate x v hempty) false r.
+  Proof.
+    intros.
+    unfold freq.
+    (* taking right branch is easy, but soundness seems difficult as we can always take it *)
+    (* right.
+    intros.
+    reflexivity. *)
+    left.
+    (* cannot prove if i take the left branch *)
+    exists hempty.
+    exists hempty.
+    repeat split.
+    rewrite hunion_empty.
+    reflexivity.
+    apply hdisjoint_empty.
+  Abort.
+
+  Example ex_take : forall x v r, (freq (contains x v)) (hupdate x v hempty) (hempty) false r.
+  Proof.
+    intros.
+    unfold freq.
+    left.
+    exists (hupdate x v hempty).
+    exists hempty.
+    repeat split.
+    rewrite hunion_comm.
+    rewrite hunion_empty.
+    reflexivity.
+    HDISJ.
+    HDISJ.
+    (* we can't say false if we take the left branch *)
+  Abort.
+
+  Example ex_vacuous_req_wrong : forall x v r, (freq (contains x v)) (hupdate x v hempty) (hempty) false r.
+  Proof.
+    intros.
+    unfold freq.
+    right.
+    (* we can always take the right branch though *)
+    intros.
+    reflexivity.
+  Qed.
+
+  Example ex_vacuous_seq : forall x v r, (freq (contains x v) ;; fens (fun r => contains x v)) (hempty) (hupdate x v hempty) false r.
+  Proof.
+    intros.
+    unfold fseq.
+    right.
+    unfold freq.
+    right.
+    intros.
+    reflexivity.
+  Qed.
+
+  Inductive forward : com -> flow -> Prop :=
+    | fw_skip:
+      forward SKIP fempty
+    | fw_pure: forall n,
+      forward (PURE n) (fens (fun res => pure (res = n)))
+    | fw_get: forall l v, 
+      forward (GET l)
+        (freq (contains l v) ;;
+        (fens (fun r => (r = v) //\\ contains l v)))
+        .
+
+  Definition terminated (c: com) : Prop :=  c = SKIP.
+
+  Definition terminates (c1: com) (h1 h2: heap) : Prop :=
+    exists c2, star red (c1, h1) (c2, h2) /\ terminated c2.
+
+  (* Definition goeswrong (c1: com) (h1: heap) : Prop :=
+    exists c2 h2, star red (c1, h1) (c2, h2) /\ error c2 h2. *)
+
+  (* Fixpoint error (c: com) (s: heap) : Prop :=
+    match c with
+    | ASSERT b => beval b s = false
+    | (c1 ;; c2) => error c1 s
+    | _ => False
+    end. *)
+
+Ltac destr H :=
+  match type of H with
+  | ex _ => 
+    let L := fresh "e" in
+    let R := fresh "H" in
+    destruct H as [L R]; destr R
+  | _ /\ _ => 
+    let L := fresh "L" in
+    let R := fresh "R" in
+    destruct H as [L R]; destr L; destr R
+  | _ => idtac
+  end.
+
+  Theorem soundness : forall c1 h1 h2 h3 r p f,
+    forward c1 f ->
+    terminates c1 h1 h2 ->
+    f h1 h3 p r ->
+    h2 = h3.
+  Proof.
+    (* intros c1. *)
+    (* induction c1; intros. *)
+    intros c1 h1 h2 h3 r p f Hf.
+    induction Hf; intros Hr Hs.
+    -
+      (* skip *)
+    {
+    inv Hr.
+    destruct H.
+    inv H.
+    -
+    (* skip has terminated *)
+      inv H0.
+      unfold fempty in Hs.
+      unfold fens in Hs.
+      destruct Hs as [h0 [H1 [H2 H3]]].
+      subst.
+      rewrite hunion_comm.
+      rewrite -> hunion_empty.
+      auto.
+      rewrite hdisjoint_sym.
+      auto.
+    -
+    (* skip reduces *)
+    inv H1.
+    }
+    -
+    (* pure *)
+    {
+      inv Hr.
+      destruct H. inv H.
+      -
+      (* pure terminates *)
+      unfold fens in Hs.
+      destruct Hs as [h0 [H1 [H2 H3]]].
+      unfold pure in H1.
+      destruct H1.
+      subst.
+      rewrite hunion_comm.
+      rewrite hunion_empty.
+      auto.
+      apply hdisjoint_empty.
+      -
+      (* pure takes steps *)
+      inv H1.
+    }
+    -
+    (* deref *)
+    {
+    inv Hr.
+    destruct H.
+    inv H.
+    -
+    (* get has terminated *)
+    inv H0.
+    - {
+    (* get reduces *)
+    inv H1.
+    inv H2.
+    - {
+    (* pure has terminated *)
+    unfold fseq in Hs.
+    destruct Hs.
+    - {
+      (* seq does not vacuously succeed early *)
+      destr H.
+      unfold freq in L.
+      destr L.
+      destruct L.
+      - destr H. unfold fens in R. destr R. subst.
+      unfold pureconj in L3. destruct L3. subst.
+      unfold contains in H1.
+      unfold contains in L1.
+      subst.
+      rewrite hunion_comm; auto.
+      -
+      pose proof (H h2 h3).
+      destr H1.
+      (* inv R0. *)
+      admit.
+    }
+    -
+      (* seq vacuously succeeds early *)
+      { inv H0.
+      inv H.
+      destruct H0.
+      destruct H.
+      - destr H. inv R0.
+      - admit.
+      }
+    } 
+    -
+    (* pure reduces *)
+    inv H.
+}
+    }
+  (* Qed. *)
+  Admitted.
+
+End Flow2.
